Tidied most laws except R2 sequential composition.

theories/theories/csp/utp_csp_laws.thy
@@ -11,13 +11,32 @@ imports
   utp_csp_healths
 begin
 
+
+lemmas R_commutes = R1_R2_commute R1_R3c_commute R2_R3c_commute
+lemmas CSP_R_commutes = CSP1_R1_commute CSP1_R2_commute CSP1_R3c_commute CSP2_R1_commute CSP2_R2_commute CSP2_R3c_commute
+lemmas R_idempotents = R1_idempotent R2_idempotent R3c_idempotent
+
+lemma RHc_idempotent:
+  "`RHc(RHc(P))` = `RHc(P)`"
+by(simp add: R_commutes R_idempotents RHc_def)
+
+lemma DesignD_pre: 
+  assumes "{ok\<down>\<acute>} \<sharp> A"  "{ok\<down>\<acute>} \<sharp> B"
+  shows "`(A \<turnstile> B)[false / ok\<acute>]` = `(\<not> $ok \<or> \<not> A)`"
+by(simp add:DesignD_def usubst typing defined closure SubstP_VarP_single_UNREST assms demorgan2)
+
+lemma DesignD_post: 
+  assumes "{ok\<down>\<acute>} \<sharp> A"  "{ok\<down>\<acute>} \<sharp> B"
+  shows "`(A \<turnstile> B)[true / ok\<acute>]` = `($ok \<and>  A) \<Rightarrow> B`"
+by(simp add:DesignD_def usubst typing defined closure SubstP_VarP_single_UNREST assms)
+
 definition CSP_Pre
   :: "'a upred \<Rightarrow> 'a upred " where
-"CSP_Pre P = `\<not>P\<^sup>f[true/ok]\<^sub>f`"
+"CSP_Pre P = `\<not>P\<^sup>f\<^sub>f[true/ok]`"
 
 definition CSP_Post
   :: "'a upred \<Rightarrow> 'a upred " where
-"CSP_Post P = `P\<^sup>t[true/ok]\<^sub>f`"
+"CSP_Post P = `P\<^sup>t\<^sub>f[true/ok]`"
 
 subsection {* Closure laws *}
 
@@ -36,97 +55,100 @@ subsection {* CSP laws *}
 lemma CSP_is_CSP1:
   assumes "P is CSP"
   shows "P is CSP1"
-proof-
-from assms have 1: "P = CSP(P)" by(metis is_healthy_def)
-show ?thesis 
-  apply(subst 1)
-  apply(simp add:is_healthy_def CSP_def CSP1_idempotent)
-  done
-qed
+by (metis CSP1_idempotent CSP_def assms comp_apply is_healthy_def)
 
 lemma CSP_is_CSP2:
   assumes "P is CSP"
   shows "P is CSP2"
-proof-
-from assms have 1: "P = CSP(P)" by(metis is_healthy_def)
-show ?thesis 
-  apply(subst 1)
-  apply(simp add:is_healthy_def CSP_def CSP1_CSP2_commute CSP2_idempotent)
-  done
-qed
+by (metis CSP1_CSP2_commute CSP_def H2_idempotent assms comp_apply is_healthy_def)
 
 lemma CSP_is_RHc: 
 assumes "P is CSP"
 shows "P is RHc" 
 proof -
-  from assms have 1: "P = CSP(P)" 
-    by (metis Healthy_simp)
-  have 2: "CSP(P) is RHc"
-    apply(simp add:is_healthy_def)
-    apply(simp add:CSP_def RHc_def)
-    apply(simp add:CSP2_R1_commute CSP2_R2_commute CSP2_R3c_commute assms closure)
-    apply(simp add:CSP1_R1_commute CSP1_R2_commute CSP1_R3c_commute)
-    apply(simp add:R1_R2_commute R1_R3c_commute R1_idempotent)
-    apply(simp add:R2_R3c_commute R2_idempotent R3c_idempotent)
-    done
-  show ?thesis 
-    by (metis "1" "2")
+  have "CSP P is RHc"
+   by(simp add:is_healthy_def CSP_def RHc_def CSP_R_commutes R_commutes R_idempotents)
+  thus ?thesis
+      by(subst Healthy_simp[THEN sym, of _ "CSP"],simp_all add: assms)
 qed
 
 lemma CSP_form: 
 assumes "P is CSP" 
-shows "P = `(\<not>$ok \<and> ($tr \<le> $tr\<acute>)) \<or> ($ok \<and> $wait \<and> II) \<or> ($ok \<and> \<not>$wait \<and> R2(\<not>CSP_Pre(P))) \<or> ($ok \<and> \<not>$wait \<and> $ok\<acute> \<and> R2(CSP_Post(P)))`"
+shows "P = `(\<not>$ok \<and> ($tr \<le> $tr\<acute>)) \<or> ($ok \<and> $wait \<and> II) \<or> 
+            ($ok \<and> \<not>$wait \<and> R2(\<not>CSP_Pre(P))) \<or> ($ok \<and> \<not>$wait \<and> $ok\<acute> \<and> R2(CSP_Post(P)))`"
 proof-
-  have "P = `($ok \<and> $wait \<and> P) \<or> ($ok \<and> \<not>$wait \<and> P) \<or> (\<not>$ok \<and> P)`"
-  by(simp add: OrP_assoc AndP_OrP_distr[THEN sym] AndP_OrP_distl[THEN sym] OrP_excluded_middle)
-  also have "... = `($ok \<and> $wait \<and> R3c(P)) \<or> ($ok \<and> \<not>$wait \<and> R2(CSP2(P))) \<or> (\<not>$ok \<and> CSP1(P))`"
-  by(metis assms is_healthy_def CSP_is_CSP1 CSP_is_CSP2 CSP_is_RHc RHc_is_R2 RHc_is_R3c)
-  also have "... = `(\<not>$ok \<and> ($tr \<le> $tr\<acute>)) \<or> ($ok \<and> $wait \<and> II) \<or> ($ok \<and> \<not>$wait \<and> R2(P\<^sup>f)) \<or> ($ok \<and> \<not>$wait \<and>  $ok\<acute> \<and> R2(P\<^sup>t))`"
-  apply(simp add:R3c_form H2_split R2s_OrP R2_def R2s_AndP R1_OrP R1_extend_AndP[THEN sym])
-  apply(simp add:R2_def[THEN sym],simp add:R2s_def usubst typing defined closure)
-  apply(subst CSP1_R1_form_2,simp_all add:assms CSP_is_RHc RHc_is_R1 CSP1_def)
-  apply(utp_poly_auto_tac)
-  done
-  also have "... =   `(\<not>$ok \<and> ($tr \<le> $tr\<acute>)) \<or> ($ok \<and> $wait \<and> II) \<or> ($ok \<and> \<not>$wait \<and> R2(\<not>CSP_Pre(P))) \<or> ($ok \<and> \<not>$wait \<and> $ok\<acute> \<and> R2(CSP_Post(P)))`"
-  apply(subst PVarPE_PSubstPE,simp add:typing) back back
-  apply(subst PVarPE_PSubstPE,simp add:typing) back back back
-  apply(simp add:usubst typing defined closure R2_ok_true)
-  apply(subst NotP_PVarPE_PSubstPE,simp_all add:typing) back
-  apply(subst NotP_PVarPE_PSubstPE,simp_all add:typing) back back
-  apply(simp add:usubst typing defined closure R2_wait_false CSP_Pre_def CSP_Post_def)
-  done
+  have "P = `(\<not>$ok \<and> P) \<or> ($ok \<and> $wait \<and> P) \<or> ($ok \<and> \<not>$wait \<and> P)`"
+    by(simp add: OrP_comm AndP_OrP_distr[THEN sym] AndP_OrP_distl[THEN sym] OrP_excluded_middle)
+  also have "... = `(\<not>$ok \<and> CSP1(R1(P))) \<or> ($ok \<and> $wait \<and> R3c(P)) \<or> ($ok \<and> \<not>$wait \<and> R2(CSP2(P)))`"
+    by(metis assms is_healthy_def CSP_is_CSP1 CSP_is_CSP2 CSP_is_RHc RHc_is_R2 RHc_is_R3c RHc_is_R1)
+  also have "... = `(\<not>$ok \<and> ($tr \<le> $tr\<acute>)) \<or> ($ok \<and> $wait \<and> R3c(P)) \<or> 
+                    ($ok \<and> \<not>$wait \<and> R2(CSP2(P)))`"
+    by(simp add:CSP1_def R1_def AndP_OrP_distl AndP_assoc AndP_OrP_distr[THEN sym] 
+        OrP_comm OrP_AndP_absorb)
+  also have "... = `(\<not>$ok \<and> ($tr \<le> $tr\<acute>)) \<or> ($ok \<and> $wait \<and> II) \<or> 
+                    ($ok \<and> $wait \<and>\<not>$ok \<and> ($tr \<le> $tr\<acute>)) \<or> ($ok \<and> \<not>$wait \<and> R2(CSP2(P)))`"
+    by(simp add: R3c_def CondR_true_cond CSP1_def AndP_OrP_distl OrP_assoc[THEN sym])
+  also have "... = `(\<not>$ok \<and> ($tr \<le> $tr\<acute>)) \<or> ($ok \<and> $wait \<and> II) \<or> ($ok \<and> \<not>$wait \<and> R2(CSP2(P)))`"
+    by(utp_poly_auto_tac)
+  also have "... = `(\<not>$ok \<and> ($tr \<le> $tr\<acute>)) \<or> ($ok \<and> $wait \<and> II) \<or> 
+                    ($ok \<and> \<not>$wait \<and> R2(P\<^sup>f)) \<or> ($ok \<and> \<not>$wait \<and> R2(P\<^sup>t \<and> $ok\<acute>))`"
+    by(simp add:H2_split R2_OrP AndP_OrP_distl)
+  also have "... = `(\<not>$ok \<and> ($tr \<le> $tr\<acute>)) \<or> ($ok \<and> $wait \<and> II) \<or> 
+                    ($ok \<and> \<not>$wait \<and> R2(P\<^sup>f)) \<or> ($ok \<and> \<not>$wait \<and> R2(P\<^sup>t) \<and> $ok\<acute>)`"
+    by(utp_poly_auto_tac)
+  also have "... = `(\<not>$ok \<and> ($tr \<le> $tr\<acute>)) \<or> ($ok \<and> $wait \<and> II) \<or> 
+                    ($ok \<and> (\<not>$wait \<and> R2(P\<^sup>f)[false/wait])[true/ok]) \<or> 
+                    ($ok \<and> (\<not>$wait \<and> (R2(P\<^sup>t) \<and> $ok\<acute>)[false/wait])[true/ok])`"
+    by(simp add: PVarPE_PSubstPE[THEN sym] NotP_PVarPE_PSubstPE[THEN sym] typing)
+  also have "... =   `(\<not>$ok \<and> ($tr \<le> $tr\<acute>)) \<or> ($ok \<and> $wait \<and> II) \<or> 
+                      ($ok \<and> \<not>$wait \<and> R2(\<not>CSP_Pre(P))) \<or> ($ok \<and> \<not>$wait \<and> R2(CSP_Post(P)) \<and> $ok\<acute>)`"
+    by(simp add:usubst typing defined closure R2_ok_true R2_wait_false CSP_Post_def CSP_Pre_def)
+  also have "... =   `(\<not>$ok \<and> ($tr \<le> $tr\<acute>)) \<or> ($ok \<and> $wait \<and> II) \<or> 
+                      ($ok \<and> \<not>$wait \<and> R2(\<not>CSP_Pre(P))) \<or> ($ok \<and> \<not>$wait \<and> $ok\<acute> \<and> R2(CSP_Post(P)))`"
+    by(metis AndP_comm)
 finally show ?thesis .
 qed
 
 subsection {* CSP as Reactive Designs *}
 
-lemma DesignD_form: "`(P \<turnstile> Q)` = `\<not>$ok \<or> ($ok \<and> \<not>P) \<or> ($ok \<and> P \<and> $ok\<acute> \<and> Q)`"
+lemma DesignD_form: "`(P \<turnstile> Q)` = `\<not>$ok \<or> ($ok \<and> \<not>P) \<or> ($ok \<and> $ok\<acute> \<and> Q)`"
 by(utp_pred_auto_tac)
+
+lemma DesignREA_form: 
+  "`RHc( P \<turnstile> Q)` = `(\<not>$ok \<and> ($tr \<le> $tr\<acute>)) \<or> ($ok \<and> $wait \<and> II) \<or> ($ok \<and> \<not>$wait \<and> R2(\<not>P)) \<or> ($ok \<and> \<not>$wait \<and> $ok\<acute> \<and> R2(Q))`"
+proof-
+  have "`RHc( P \<turnstile> Q)` =  `R2 ((\<not> $ok \<and> $wait \<and> ($tr \<le> $tr\<acute>)) \<or> ($ok \<and> $wait \<and> II) \<or> (\<not> $wait \<and> (P \<turnstile> Q)))`"
+    by(simp add:RHc_def R3c_form NotP_PVarPE_PSubstPE[THEN sym] typing R2_def R1_idempotent)
+  also have "... = `(\<not> $ok \<and> $wait \<and> ($tr \<le> $tr\<acute>)) \<or> ($ok \<and> $wait \<and> R2(II)) \<or> (\<not> $wait \<and> R2(P \<turnstile> Q))`"
+    by(simp add:R2_def R2s_def usubst typing defined closure R1_def AndP_OrP_distr AndP_assoc[THEN sym])
+  also have "... = `(\<not> $ok \<and> $wait \<and> ($tr \<le> $tr\<acute>)) \<or> ($ok \<and> $wait \<and> II) \<or> (\<not> $wait \<and> R2(P \<turnstile> Q))`"
+    by(simp add:SkipRA_is_R2)
+  also have "... = `(\<not>$ok \<and> $wait\<and> ($tr \<le> $tr\<acute>)) \<or> ($ok \<and> $wait \<and> II) \<or> (\<not>$wait \<and> \<not>$ok \<and>($tr \<le> $tr\<acute>)) \<or> (\<not>$wait \<and> $ok \<and> R2(\<not>P)) \<or> (\<not>$wait \<and> $ok \<and> $ok\<acute> \<and> R2(Q))`"
+    by(simp add: DesignD_form R2_def R2s_def usubst typing defined closure R1_def AndP_OrP_distr AndP_OrP_distl AndP_assoc[THEN sym])
+  also have "... = `(\<not>$ok \<and> ($tr \<le> $tr\<acute>)) \<or> ($ok \<and> $wait \<and> II) \<or> ($ok \<and> \<not>$wait \<and> R2(\<not>P)) \<or> ($ok \<and> \<not>$wait \<and> $ok\<acute> \<and> R2(Q))`"
+    by(utp_poly_auto_tac)
+  finally show ?thesis .
+qed
 
 lemma CSP_Design: 
 assumes "P is CSP" 
 shows "P = `RHc ( CSP_Pre(P) \<turnstile> CSP_Post(P))`"
-apply(subst CSP_form, simp_all add: assms)
-apply(simp add:DesignD_form RHc_def R2_R3c_commute)
-apply(simp add: R2_def R2s_def usubst typing defined closure R3c_def SkipR_as_SkipRA)
-apply(subst SkipRA_unfold_aux_ty[of "tr"],simp_all add:typing defined closure)
-apply(subst SkipRA_unfold_aux_ty[of "tr"],simp_all add:typing defined closure) back
-apply(utp_poly_auto_tac)
-done
+  by(simp add:DesignREA_form assms CSP_form[simplified,THEN sym])
 
-lemma DesignREA_form: 
-  "`RHc( P \<turnstile> Q)` = `(\<not>$ok \<and> ($tr \<le> $tr\<acute>)) \<or> ($ok \<and> $wait \<and> II) \<or> ($ok \<and> \<not>$wait \<and> R2(\<not>P)) \<or> ($ok \<and> \<not>$wait \<and> R2(Q) \<and> $ok\<acute>)`"
-apply(simp add:DesignD_form RHc_def R3c_form SkipR_as_SkipRA)
-apply(subst SkipRA_unfold_aux_ty[of "tr"],simp_all add:closure typing)
-apply(subst SkipRA_unfold_aux_ty[of "tr"],simp_all add:closure typing)back
-apply(simp add:R2_def R1_idempotent R2s_def usubst typing defined closure)
-apply(simp add:R1_OrP)
-apply(simp add:R1_def AndP_assoc[THEN sym])
-apply(subst AndP_assoc) back back back
-apply(subst AndP_comm) back back back back
-apply(simp add:AndP_assoc[THEN sym] tr_prefix_as_nil)
-apply(utp_poly_auto_tac)
-done
+lemma DesignREA_CSP:
+  assumes "{ok\<down>\<acute>} \<sharp> A"  "{ok\<down>\<acute>} \<sharp> B"
+  shows "`RHc (A \<turnstile> B)` is CSP"
+proof-
+  have "`CSP(RHc(A \<turnstile> B))` =  `RHc(CSP1(CSP2(A \<turnstile> B)))`"
+    by (metis (no_types) CSP_R_commutes CSP_def RHc_def RHc_idempotent comp_apply)
+  also have "... = `RHc (CSP1 ((\<not>$ok \<or> \<not> A) \<or> (($ok \<and> A) \<Rightarrow> B) \<and> $ok\<acute>))`"
+    by (simp add: H2_split DesignD_pre[simplified] DesignD_post[simplified] assms)
+  also have "... = `RHc(A \<turnstile> B)`"
+    by (utp_poly_auto_tac)
+  finally show ?thesis
+    by (metis Healthy_intro)
+qed
+
 
 lemma DesignREA_form2:  "`RHc( P \<turnstile> Q)` = `(\<not>$ok \<and> ($tr \<le> $tr\<acute>)) \<or> ($ok \<and> $wait \<and> II) \<or> ($ok \<and> \<not>$wait \<and> R2(\<not>P)) \<or> ($ok \<and> \<not>$wait \<and> \<not>R2(\<not>P) \<and> R2(Q) \<and> $ok\<acute>)`"
 by(simp add:DesignREA_form,utp_poly_auto_tac)
@@ -140,14 +162,7 @@ proof-
 from assms have "`\<not>CSP_Pre(P)` = `\<not>CSP_Pre(R2(P))`"
 by(metis is_healthy_def)
 also have "... = `R2(\<not>CSP_Pre(P))`"
-apply(subst CSP_Pre_def)
-apply(subst R2_ok'_false)
-apply(subst R2_ok_true)
-apply(subst R2_wait_false)
-apply(subst NotP_NotP[THEN sym]) back back back back back back
-apply(subst CSP_Pre_def)
-apply(simp add: NotP_NotP)
-done
+by(simp add:CSP_Pre_def R2_ok'_false[simplified] R2_wait_false R2_ok_true)
 finally show ?thesis by(metis is_healthy_def)
 qed
 
@@ -157,13 +172,7 @@ lemma CSP_Post_R2:
 proof -
 from assms have "`CSP_Post(P)` = `CSP_Post(R2(P))`" by (metis assms is_healthy_def)
 also have "... = `R2(CSP_Post(P))`"
-apply(subst CSP_Post_def)
-apply(subst R2_ok'_true)
-apply(subst R2_ok_true)
-apply(subst R2_wait_false)
-apply(subst CSP_Post_def[THEN sym])
-apply(simp)
-done
+by(simp add:CSP_Post_def R2_ok'_true[simplified] R2_wait_false R2_ok_true)
 finally show ?thesis by(metis is_healthy_def)
 qed
 
@@ -171,23 +180,10 @@ lemma CSP_Pre_DesignREA:
   assumes "{ok\<down>}\<sharp>A" "{ok\<down>\<acute>}\<sharp>A" "{wait\<down>}\<sharp>A" "`\<not>A` is R2"
   shows "`CSP_Pre(RHc( A \<turnstile> B))` = `A`"
 proof -
-have "`CSP_Pre(RHc( A \<turnstile> B))` = `\<not>(R2(\<not>A))`"
-apply(simp add:DesignREA_form CSP_Pre_def usubst typing defined closure R2_def R1_def R2s_def)
-apply(subst SubstP_twice_3) back
-apply(simp_all add:unrest typing defined closure)
-apply(subst SubstP_twice_3) back back
-apply(simp_all add:unrest typing defined closure)
-apply(subst SubstP_twice_3) back back back
-apply(simp_all add:unrest typing defined closure)
-apply(subst SubstP_twice_3)
-apply(simp_all add:unrest typing defined closure)
-apply(subst SubstP_twice_3) back
-apply(simp_all add:unrest typing defined closure)
-apply(subst SubstP_twice_3) back back
-apply(simp_all add:unrest typing defined closure)
-apply(simp add:usubst typing defined closure)
-apply(simp add:SubstP_VarP_single_UNREST assms demorgan2 ImpliesP_def)
-done
+have "`CSP_Pre(RHc( A \<turnstile> B))` = `\<not>(R2(\<not>A[false/ok\<acute>][false/wait][true/ok]))`"
+by(simp add:DesignREA_form CSP_Pre_def usubst typing defined closure R2_ok'_false[simplified] R2_wait_false R2_ok_true)
+also have "... = `\<not>(R2(\<not>A))`"
+by(simp add:assms SubstP_VarP_single_UNREST)
 also have "... = A"
 by (metis NotP_NotP assms(4) is_healthy_def)
 finally show ?thesis .
@@ -197,26 +193,10 @@ lemma CSP_Post_DesignREA:
   assumes "{ok\<down>}\<sharp>`A\<Rightarrow>B`" "{ok\<down>\<acute>}\<sharp>`A\<Rightarrow>B`" "{wait\<down>}\<sharp>`A\<Rightarrow>B`" "`A \<Rightarrow> B` is R2"
   shows"`CSP_Post(RHc( A \<turnstile> B))` = `A \<Rightarrow> B`"
 proof -
-have "`CSP_Post(RHc( A \<turnstile> B))` = `R1(CSP_Post(R2s(A \<Rightarrow> B)))`"
-by(simp add:DesignREA_form CSP_Post_def usubst typing defined closure R2_def R1_def R2s_def AndP_OrP_distr[THEN sym] ImpliesP_def)
-also have "... = `R2(CSP_Post(A \<Rightarrow> B))`"
-apply(simp add:CSP_Post_def R2s_def)
-apply(subst SubstP_twice_3) back
-apply(simp_all add:typing defined closure unrest)
-apply(subst SubstP_twice_3) back back
-apply(simp_all add:typing defined closure unrest)
-apply(subst SubstP_twice_3) back back back
-apply(simp_all add:typing defined closure unrest)
-apply(subst SubstP_twice_3)
-apply(simp_all add:typing defined closure unrest)
-apply(subst SubstP_twice_3) back
-apply(simp_all add:typing defined closure unrest)
-apply(subst SubstP_twice_3) back back
-apply(simp_all add:typing defined closure unrest)
-apply(simp add:usubst typing defined closure R2_def R2s_def)
-done
+have "`CSP_Post(RHc( A \<turnstile> B))` = `R2((A \<Rightarrow> B)[true/ok\<acute>][false/wait][true/ok])`"
+by(simp add:DesignREA_form CSP_Post_def usubst typing defined closure R2_ok'_true[simplified] R2_wait_false R2_ok_true ImpliesP_def R2_OrP)
 also have "... = `R2(A \<Rightarrow> B)`"
-by(simp add:CSP_Post_def SubstP_VarP_single_UNREST assms)
+by(simp add:assms SubstP_VarP_single_UNREST)
 finally show ?thesis
 by (metis Healthy_simp assms(4))
 qed
@@ -224,42 +204,16 @@ qed
 lemma CSP_Pre_UNREST: 
   assumes "{ok\<down>,wait\<down>,ok\<down>\<acute>} \<sharp> `P`"
   shows "`CSP_Pre(P)` = `\<not>P`"
-apply(simp add:CSP_Pre_def)
-apply(subst SubstP_VarP_single_UNREST)
-apply(subst UNREST_subset[of "{ok\<down>,wait\<down>,ok\<down>\<acute>}"])
-apply(simp_all add:assms)
-apply(subst SubstP_VarP_single_UNREST)
-apply(subst UNREST_subset[of "{ok\<down>,wait\<down>,ok\<down>\<acute>}"])
-apply(simp_all add:assms)
-apply(subst SubstP_VarP_single_UNREST)
-apply(subst UNREST_subset[of "{ok\<down>,wait\<down>,ok\<down>\<acute>}"])
-apply(simp_all add:assms)
-done
+by(simp add:CSP_Pre_def SubstP_VarP_single_UNREST UNREST_subset[of "{ok\<down>,wait\<down>,ok\<down>\<acute>}"] assms)
 
 lemma CSP_Post_UNREST: 
   assumes "{ok\<down>,wait\<down>,ok\<down>\<acute>} \<sharp> `P`"
   shows "`CSP_Post(P)` = `P`"
-apply(simp add:CSP_Post_def)
-apply(subst SubstP_VarP_single_UNREST)
-apply(subst UNREST_subset[of "{ok\<down>,wait\<down>,ok\<down>\<acute>}"])
-apply(simp_all add:assms)
-apply(subst SubstP_VarP_single_UNREST)
-apply(subst UNREST_subset[of "{ok\<down>,wait\<down>,ok\<down>\<acute>}"])
-apply(simp_all add:assms)
-apply(subst SubstP_VarP_single_UNREST)
-apply(subst UNREST_subset[of "{ok\<down>,wait\<down>,ok\<down>\<acute>}"])
-apply(simp_all add:assms)
-done
+by(simp add:CSP_Post_def SubstP_VarP_single_UNREST UNREST_subset[of "{ok\<down>,wait\<down>,ok\<down>\<acute>}"] assms)
 
 lemma CSP_Pre_R2_commute:
   "`\<not>CSP_Pre(R2(P))` = `R2(\<not>CSP_Pre(P))`"
-apply(subst CSP_Pre_def) back
-apply(subst NotP_NotP)
-apply(subst R2_wait_false[THEN sym])
-apply(subst R2_ok_true[THEN sym])
-apply(simp add:R2_def[THEN sym] CSP_Pre_def)
-apply (metis PVAR_VAR_pvdash R2_ok'_false)
-done
+by(simp add:CSP_Pre_def R2_ok'_false[simplified] R2_wait_false R2_ok_true)
 
 lemma CSP_Post_R1_commute:
   "`CSP_Post(R1(P))` = `R1(CSP_Post(P))`"
@@ -267,11 +221,7 @@ by(simp add:CSP_Post_def R1_def usubst typing defined closure)
 
 lemma CSP_Post_R2_commute:
   "`CSP_Post(R2(P))` = `R2(CSP_Post(P))`"
-apply(simp add:CSP_Post_def)
-apply(simp add: R2_wait_false[THEN sym] R2_ok_true[THEN sym])
-apply (metis PVAR_VAR_pvdash R2_ok'_true)
-done
-
+by(simp add:CSP_Post_def R2_ok'_true[simplified] R2_wait_false R2_ok_true)
 
 lemma CSP_Pre_OrP:
   "`CSP_Pre(A \<or> B)` = `CSP_Pre(A) \<and> CSP_Pre(B)`"
@@ -343,72 +293,25 @@ done
 
 lemma DesignREA_pre:
   shows "`CSP_Pre(RHc(A \<turnstile> B))` = `\<not>R2(\<not>CSP_Pre(\<not>A))`"
-apply(subst DesignREA_form,simp add:CSP_Pre_def usubst typing defined closure)
-apply(simp add:SubstP_NotP[THEN sym])
-apply(subst SubstP_NotP)apply(subst SubstP_NotP)apply(subst SubstP_NotP)
-apply(subst R2_wait_false[THEN sym])
-apply(subst R2_ok_true[THEN sym])
-apply (metis PVAR_VAR_pvdash R2_ok'_false)
-done
+by(simp add:DesignREA_form CSP_Pre_def usubst typing defined closure R2_ok_true R2_wait_false R2_ok'_false[simplified])
 
 lemma DesignREA_post:
   shows "`CSP_Post(RHc(A \<turnstile> B))` = `R2(CSP_Post(A \<Rightarrow> B))`"
-apply(subst DesignREA_form,simp add:CSP_Post_def usubst typing defined closure ImpliesP_def)
-apply(simp add:SubstP_OrP[THEN sym] SubstP_NotP[THEN sym] R2_OrP[THEN sym])
-apply(simp add:ImpliesP_def[THEN sym])
-apply(subst R2_wait_false[THEN sym])
-apply(subst R2_ok_true[THEN sym])
-apply (metis PVAR_VAR_pvdash R2_ok'_true)
-done
-
-lemma RHc_idempotent:
-  "`RHc(RHc(P))` = `RHc(P)`"
-by(simp add: R1_R2_commute R1_R3c_commute R1_idempotent R2_R3c_commute R2_idempotent R3c_idempotent RHc_def)
-
-lemmas R_commutes = R1_R2_commute R1_R3c_commute R2_R3c_commute
-lemmas CSP_R_commutes = CSP1_R1_commute CSP1_R2_commute CSP1_R3c_commute CSP2_R1_commute CSP2_R2_commute CSP2_R3c_commute
-
-lemma DesignD_pre: 
-  assumes "{ok\<down>\<acute>} \<sharp> A"  "{ok\<down>\<acute>} \<sharp> B"
-  shows "`(A \<turnstile> B)[false / ok\<acute>]` = `(\<not> $ok \<or> \<not> A)`"
-by(simp add:DesignD_def usubst typing defined closure SubstP_VarP_single_UNREST assms demorgan2)
-
-lemma DesignD_post: 
-  assumes "{ok\<down>\<acute>} \<sharp> A"  "{ok\<down>\<acute>} \<sharp> B"
-  shows "`(A \<turnstile> B)[true / ok\<acute>]` = `($ok \<and>  A) \<Rightarrow> B`"
-by(simp add:DesignD_def usubst typing defined closure SubstP_VarP_single_UNREST assms)
-
-lemma DesignREA_CSP:
-  assumes "{ok\<down>\<acute>} \<sharp> A"  "{ok\<down>\<acute>} \<sharp> B"
-  shows "`RHc (A \<turnstile> B)` is CSP"
-proof-
-  have "`CSP(RHc(A \<turnstile> B))` =  `RHc(CSP1(CSP2(A \<turnstile> B)))`"
-    by (metis (no_types) CSP_R_commutes CSP_def RHc_def RHc_idempotent comp_apply)
-  also have "... = `RHc (CSP1 ((\<not>$ok \<or> \<not> A) \<or> (($ok \<and> A) \<Rightarrow> B) \<and> $ok\<acute>))`"
-    by (simp add: H2_split DesignD_pre[simplified] DesignD_post[simplified] assms)
-  also have "... = `RHc(A \<turnstile> B)`"
-    by (utp_poly_auto_tac)
-  finally show ?thesis
-    by (metis Healthy_intro)
-qed
+by(simp add:DesignREA_form CSP_Post_def usubst typing defined closure R2_ok_true R2_wait_false R2_ok'_true[simplified] ImpliesP_def R2_OrP)
 
 lemma DesignREA_Pre_Post:
   "`RHc(A\<turnstile>B)` = `RHc(A \<turnstile> A \<and> B)`"
 by(utp_poly_auto_tac)
 
 lemma Design_Eq:
-  assumes "A is R2s" "C is R2s" "`A` = `C`" "`A \<Rightarrow> B` = `C \<Rightarrow> D`"
+  assumes "`A` = `C`" "`A \<Rightarrow> B` = `C \<Rightarrow> D`"
   shows "`RHc(A \<turnstile> B)` = `RHc(C \<turnstile> D)`"
 proof -
   have 0: "`RHc(A \<turnstile> B)` = `RHc(C \<turnstile> (C \<Rightarrow> D))`"
-  apply(simp add:assms(3) assms(4)[THEN sym])
-  apply(simp add: DesignREA_form ImpliesP_def R2_OrP AndP_OrP_distl AndP_OrP_distr)
-  apply(subst OrP_assoc,simp add:AndP_assoc OrP_AndP_absorb) back back back back
-  done
-  show ?thesis
-  apply(subst 0, simp add: DesignREA_form ImpliesP_def R2_OrP AndP_OrP_distl AndP_OrP_distr)
-  apply(subst OrP_assoc,simp add:AndP_assoc OrP_AndP_absorb) back back 
-  done
+  by(simp add:assms(1) assms(2)[THEN sym],utp_poly_auto_tac)
+  also have "... = `RHc(C \<turnstile> D)`" 
+  by(utp_poly_auto_tac)
+  finally show ?thesis .
 qed
 
 subsection {* Sequential composition *}
@@ -419,7 +322,7 @@ lemma left_form_P:
   (\<not>$ok \<and> ($tr \<le> $tr\<acute>)) \<or> 
   ($ok \<and> $wait \<and> II) \<or> 
   ($ok \<and> \<not>$wait \<and> R2(\<not>CSP_Pre(P))) \<or> 
-  ($ok \<and> \<not>$wait \<and> R2(CSP_Post(P)) \<and> $ok\<acute>)`"
+  ($ok \<and> \<not>$wait \<and> $ok\<acute>\<and> R2(CSP_Post(P)) )`"
   by(subst CSP_Design,simp_all add: DesignREA_form assms)
 
 lemma Seq_comp_1: 
@@ -428,18 +331,13 @@ lemma Seq_comp_1:
 proof -
   have "`(\<not>$ok \<and> ($tr \<le> $tr\<acute>));Q` = `(\<not>$ok \<and> ($tr \<le> $tr\<acute>));CSP1(R1(Q))`"
     by(metis assms is_healthy_def CSP_is_CSP1 CSP_is_RHc RHc_is_R1)
+  also have "... = `\<not>$ok \<and> ($tr \<le> $tr\<acute>);((Q \<or> \<not> $ok) \<and> ($tr \<le> $tr\<acute>))`"
+    by(simp add: SemiR_AndP_left_precond closure typing defined assms CSP1_def R1_def AndP_OrP_distr[THEN sym])
+  also have "... = `\<not>$ok \<and> ($tr \<le> $tr\<acute>) ; ($tr\<le>$tr\<acute>)`"
+    by(simp add:AndP_OrP_distr SemiR_OrP_distl SemiR_remove_middle_unrest1[of _ _ "{ok \<down>}" "`\<not>$ok`"] typing closure defined assms unrest R1_def,utp_poly_auto_tac)
   also have "... = `\<not>$ok \<and> ($tr \<le> $tr\<acute>)`"
-    apply(subst SemiR_AndP_left_precond,simp_all add:closure typing defined assms)
-    apply(subst CSP1_R1_form, simp add:is_healthy_def R1_idempotent)
-    apply(simp add:CSP1_def SemiR_OrP_distl)
-    apply(subst SemiR_remove_middle_unrest1[of _ _ "{ok \<down>}"],simp_all add:typing closure defined assms unrest)
-    apply(subst SemiR_remove_middle_unrest1[of _ _ "{ok \<down>}"],simp_all add:typing closure defined unrest)
-    apply(simp add:R1_def usubst typing defined closure SemiR_OrP_distl[THEN sym])
-    apply(subst tr_leq_trans[THEN sym]) back back back
-    apply(utp_poly_auto_tac)
-    done
-  finally show ?thesis
-    by this
+    by (metis tr_leq_trans)
+  finally show ?thesis .
 qed
 
 lemma Seq_comp_2: 
@@ -447,11 +345,7 @@ lemma Seq_comp_2:
   shows "`($ok \<and> $wait \<and> II);Q` = `$ok \<and> $wait \<and> II`"
 proof -
   have "`($ok \<and> $wait \<and> II);Q` =`($ok \<and> $wait \<and> II\<^bsub>REL_VAR - OKAY - {wait \<down>,wait \<down>\<acute>}\<^esub>);($ok \<and> $wait \<and> Q)`"
-    apply(simp add:SkipR_as_SkipRA SemiR_AndP_right_precond typing closure urename assms AndP_assoc[THEN sym])
-    apply(subst SkipRA_unfold_aux_ty[of "ok"], simp_all add:closure typing)
-    apply(subst SkipRA_unfold_aux_ty[of "wait"], simp_all add:closure typing)
-    apply(utp_poly_auto_tac)
-    done
+    by(simp add:SkipR_as_SkipRA SemiR_AndP_right_precond typing closure urename assms AndP_assoc[THEN sym] SkipRA_unfold_aux_ty[of "ok"] SkipRA_unfold_aux_ty[of "wait"],utp_poly_auto_tac)
   also have "... = `($ok \<and> $wait \<and> II\<^bsub>REL_VAR - OKAY - {wait \<down>,wait \<down>\<acute>}\<^esub>);($ok \<and> $wait \<and> R3c(Q))`"
     proof -
       have 1: "Q = `R3c(Q)`"
@@ -460,39 +354,26 @@ proof -
         by(subst 1,simp)
     qed
   also have "... = `($ok \<and> $wait \<and> II\<^bsub>REL_VAR - OKAY - {wait \<down>,wait \<down>\<acute>}\<^esub>);($ok \<and> $wait \<and> II)`"
-    apply(simp add:R3c_def CSP1_def)
-    apply(utp_poly_auto_tac)
-    done
+    by(utp_poly_auto_tac)
   also have "... = `($ok \<and> $wait \<and> II\<^bsub>REL_VAR - OKAY - {wait \<down>,wait \<down>\<acute>}\<^esub> \<and> $ok\<acute> \<and> $wait\<acute>)`"
     by(simp add:SemiR_AndP_right_precond assms closure typing urename AndP_assoc[THEN sym])
   also have "... = `$ok \<and> $wait \<and> II`"
-    apply(simp add:SkipR_as_SkipRA)
-    apply(subst SkipRA_unfold_aux_ty[of "ok"], simp_all add:closure typing) back
-    apply(subst SkipRA_unfold_aux_ty[of "wait"], simp_all add:closure typing) back
-    apply(utp_poly_auto_tac)
-    done
-  finally show ?thesis
-    by this
+    by(simp add:SkipR_as_SkipRA SkipRA_unfold_aux_ty[of "ok"] SkipRA_unfold_aux_ty[of "wait"] closure typing,utp_poly_auto_tac)
+  finally show ?thesis .
 qed
 
 lemma Seq_comp_3: 
   assumes "Q is CSP" "Q\<in> WF_RELATION" "P\<in> WF_RELATION"
   shows "`($ok \<and> \<not>$wait \<and> R2(\<not>CSP_Pre(P)));Q` = `$ok \<and> \<not>$wait \<and> (R2(\<not>CSP_Pre(P));($tr\<le>$tr\<acute>))`"
 proof -
+  have 0: "{ok\<down>\<acute>} \<sharp> `R2 (\<not> CSP_Pre(P))`" 
+    by(simp add:R2_def CSP_Pre_def unrest typing defined closure assms R1_def R2s_def)
   have "`($ok \<and> \<not>$wait \<and> R2(\<not>CSP_Pre(P)));Q` = `($ok \<and> \<not>$wait \<and> R2(\<not>CSP_Pre(P)));CSP1(R1(Q))`"
     by(metis assms is_healthy_def CSP_is_CSP1 CSP_is_RHc RHc_is_R1)
+  also have "... = `($ok \<and> \<not> $wait \<and> R2 (\<not> CSP_Pre(P)) ; CSP1 ($ok \<and> R1(Q)[true/ok]))`"
+    by(simp add: SemiR_AndP_left_precond closure typing defined assms,subst CSP1_R1_form, simp_all add:is_healthy_def R1_idempotent)
   also have "... = `$ok \<and> \<not>$wait \<and> (R2(\<not>CSP_Pre(P));($tr\<le>$tr\<acute>))`"
-    apply(subst SemiR_AndP_left_precond,simp_all add:closure typing defined assms)
-    apply(subst SemiR_AndP_left_precond,simp_all add:closure typing defined assms)
-    apply(subst CSP1_R1_form, simp add:is_healthy_def R1_idempotent)
-    apply(simp add:CSP1_def SemiR_OrP_distl)
-    apply(subst SemiR_remove_middle_unrest1[of _ _ "{ok \<down>}"],simp_all add:typing closure defined assms unrest)
-    apply(simp add:typing closure defined assms unrest CSP_Pre_def R2_def R2s_def R1_def)
-    apply(subst SemiR_remove_middle_unrest1[of _ _ "{ok \<down>}"],simp_all add:typing closure defined unrest assms)
-    apply(simp add:typing closure defined assms unrest CSP_Pre_def R2_def R2s_def R1_def)
-    apply(simp add:R1_def usubst typing defined closure SemiR_OrP_distl[THEN sym] AndP_assoc[THEN sym])
-    apply(utp_poly_auto_tac)
-    done
+    by(simp add:CSP1_def SemiR_OrP_distl SemiR_remove_middle_unrest1[of "`R2(\<not>CSP_Pre(P))`" _ "{ok \<down>}"] 0 typing closure defined assms unrest,utp_poly_auto_tac)
   finally show ?thesis
     by this
 qed
@@ -504,16 +385,7 @@ proof -
 have 0: 
   "P is R1" "P is R2" "P is R3c" "P is CSP1"
   "Q is R1" "Q is R2" "Q is R3c" "Q is CSP1" "Q is CSP2"
-  apply(metis assms CSP_is_RHc RHc_is_R1)
-  apply(metis assms CSP_is_RHc RHc_is_R2)
-  apply(metis assms CSP_is_RHc RHc_is_R3c)
-  apply(metis assms CSP_is_CSP1)
-  apply(metis assms CSP_is_RHc RHc_is_R1)
-  apply(metis assms CSP_is_RHc RHc_is_R2)
-  apply(metis assms CSP_is_RHc RHc_is_R3c)
-  apply(metis assms CSP_is_CSP1)
-  apply(metis assms CSP_is_CSP2)
-done
+  by(metis assms CSP_is_RHc RHc_is_R1 RHc_is_R2 RHc_is_R3c CSP_is_CSP1 CSP_is_CSP2)+
 have 1: "`P;Q` is R1" 
   by(simp add: 0 R1_SemiR_closure assms)
 have 2: "`P;Q` is R2" 
@@ -524,10 +396,10 @@ have 4: "`P;Q` is CSP1"
   by(simp add: 0 CSP1_SemiR_closure assms)
 have 5: "`P;Q` is CSP2" 
   by(simp add: 0 CSP2_SemiR_closure assms)
-show ?thesis
-apply(simp add: is_healthy_def CSP_def RHc_def)
-apply(metis 1 2 3 4 5 is_healthy_def)
-done
+have "`CSP1 (CSP2 (R1 (R2 (R3c (P ; Q)))))` = `(P ; Q)`"
+by(metis 1 2 3 4 5 is_healthy_def CSP_def RHc_def)
+thus ?thesis
+by(simp add: is_healthy_def CSP_def RHc_def)
 qed
 
 end
