theories/theories/csp/utp_csp_healths.thy
@@ -117,19 +117,20 @@ lemma CSP1_SemiR_closure:
   assumes "P is CSP1" "Q is CSP1" "Q is R1"
   shows " `P ; Q` is CSP1"
 proof -
-have "`P ; Q` = `CSP1(P);Q`" by (metis assms is_healthy_def)
-also have "... = `(P;Q) \<or> (\<not>$ok \<and> ($tr \<le> $tr\<acute>));R1(CSP1(Q))`" 
-apply(subst CSP1_def, simp add: SemiR_OrP_distr)
-apply(metis assms is_healthy_def)
-done
-also have "... = ` (P ; Q) \<or> (\<not> $ok \<and> ($tr \<le> $tr\<acute>)) ; ((Q \<or> true) \<and> ($tr \<le> $tr\<acute>))`"
-apply(subst AndP_OrP_distr)
-apply(simp add:R1_def CSP1_def AndP_OrP_distr AndP_assoc[THEN sym] SemiR_OrP_distl)
-apply(subst SemiR_remove_middle_unrest1[of _ _ "{ok \<down>}"],simp_all add:typing closure unrest) back
-done
-also have "... = `CSP1(P ; Q)`"
-by(simp add:SemiR_AndP_left_precond typing closure defined tr_leq_trans CSP1_def)
-finally show ?thesis by (metis is_healthy_def)
+  have "`P ; Q` = `CSP1(P);Q`" 
+    by (metis assms is_healthy_def)
+  also have "... = `(P;Q) \<or> (\<not>$ok \<and> ($tr \<le> $tr\<acute>));Q`" 
+    by(subst CSP1_def, simp add: SemiR_OrP_distr)
+  also have "... = `(P;Q) \<or> (\<not>$ok \<and> ($tr \<le> $tr\<acute>));R1(CSP1(Q))`" 
+    by(metis assms is_healthy_def)
+  also have "... = `(P ; Q \<or> (\<not> $ok \<and> ($tr \<le> $tr\<acute>)) ; (Q \<and> ($tr \<le> $tr\<acute>)) \<or> (\<not> $ok \<and> ($tr \<le> $tr\<acute>)) ; ($tr \<le> $tr\<acute>))`"
+    by(simp add:R1_def CSP1_def AndP_OrP_distr AndP_assoc[THEN sym] SemiR_OrP_distl SemiR_remove_middle_unrest1[of _ _ "{ok \<down>}"] typing closure unrest)
+  also have "... = `(P ; Q \<or> (\<not> $ok \<and> ($tr \<le> $tr\<acute>)) ; ($tr \<le> $tr\<acute>))`"
+    by(utp_poly_auto_tac)
+  also have "... = `CSP1(P;Q)`"
+    by(simp add:SemiR_AndP_left_precond typing closure defined tr_leq_trans CSP1_def[THEN sym])
+  finally show ?thesis 
+    by (metis is_healthy_def)
 qed
 
 subsection {* CSP2 laws *}
@@ -151,25 +152,51 @@ by(simp add:H2_split R1_def usubst typing defined closure,utp_pred_auto_tac)
 
 lemma CSP2_R2_commute:
   "CSP2 (R2 P) = R2 (CSP2 (P))"
-apply(simp add:H2_split R2_OrP)
-apply(subst R2_def) back back back
-apply(simp add:R2s_AndP R1_extend_AndP[THEN sym])
-apply(simp add:R2_def[THEN sym])
-apply(simp add:R2s_def usubst typing defined closure)
-apply (metis (hide_lams, no_types) PVAR_VAR_pvdash R2_ok'_false R2_ok'_true)
-done
+proof-
+  have "R2( CSP2 P) = `R2 (P\<^sup>f) \<or> R2 (P\<^sup>t) \<and> R2s ($ok\<acute>)`"
+      by(simp add:H2_split R1_OrP R1_extend_AndP R2s_AndP R2s_OrP R2_def)
+  also have "... = `R2 (P)\<^sup>f \<or> R2 (P)\<^sup>t \<and> $ok\<acute>`"
+      by(simp add: R2_ok'_true[simplified]  R2_ok'_false[simplified] R2s_def usubst typing defined closure)
+  also have "... = CSP2 (R2 P)"
+      by(simp add:H2_split)
+  finally show ?thesis ..
+qed
+
 
 lemma CSP1_SkipR: "`CSP1(II)` = `(\<not>$ok \<and> ($tr \<le> $tr\<acute>)) \<or> ($ok \<and> $ok\<acute> \<and> II\<^bsub>REL_VAR - OKAY\<^esub>)`"
-apply(simp add:R1_SkipR is_healthy_def CSP1_R1_form,simp add: SkipR_as_SkipRA)
-apply(subst SkipRA_unfold_aux_ty[of "ok"], simp_all add:usubst typing defined closure)
-apply(utp_poly_auto_tac)
-done
+proof -
+  have "`CSP1(II)` = `CSP1($ok \<and> II[true/ok])`"
+    by(simp add:closure CSP1_R1_form)
+  also have "... = `CSP1 ($ok \<and> (($ok\<acute> = $ok) \<and> II\<^bsub>REL_VAR - OKAY\<^esub>)[true/ok])`"
+    by(simp add:SkipRA_unfold_aux_ty[of "ok"] closure typing defined SkipR_as_SkipRA)
+  also have "... = `CSP1($ok \<and> $ok\<acute>=true \<and> II\<^bsub>REL_VAR - OKAY\<^esub>)`"
+    by(simp add:usubst typing defined closure)
+  also have "... = `CSP1($ok \<and> $ok\<acute> \<and> II\<^bsub>REL_VAR - OKAY\<^esub>)`"
+    by(utp_poly_auto_tac)
+  finally show ?thesis by(simp add:CSP1_def OrP_comm)
+qed
 
 lemma CSP2_R3c_commute: 
   "CSP2 (R3c P) = R3c (CSP2 (P))"
-apply(simp add:H2_split usubst typing closure defined CSP1_SkipR R3c_def)
-apply(utp_poly_auto_tac)
-done
+proof - 
+have 0: "CSP1 II is CSP2"
+proof -
+  have "`CSP2(CSP1(II))` = `(\<not> $ok \<and> ($tr \<le> $tr\<acute>)) \<or> ($ok \<and> II\<^bsub>REL_VAR - OKAY\<^esub> \<and> $ok\<acute>)`"
+    by(simp add:CSP1_SkipR H2_split usubst typing defined closure AndP_OrP_distr OrP_assoc OrP_AndP_absorb AndP_assoc)
+  also have "... = `CSP1(II)`"
+    by(simp add:CSP1_SkipR AndP_comm)
+  finally show ?thesis by (metis is_healthy_def)
+qed
+have "CSP2(R3c P) = `(($wait \<and> CSP1(II)) ; J \<or> (\<not> $wait \<and> P) ; J)`"
+by(simp add:H2_def R3c_def CondR_def SemiR_OrP_distr)
+also have "... = `(($wait \<and> CSP1(II) ; J) \<or> \<not> $wait \<and> P ; J)`"
+by(simp add: SemiR_AndP_left_DASHED unrest typing defined closure)
+also have "... = `(($wait \<and> CSP1(II)) \<or> \<not> $wait \<and> P ; J)`"
+by(metis H2_def[THEN sym] is_healthy_def 0)
+also have "... = R3c(CSP2 P)"
+by(simp add:H2_def R3c_def CondR_def SemiR_OrP_distr)
+finally show ?thesis .
+qed
 
 lemma CSP2_SemiR_closure:
   assumes "Q is CSP2"
@@ -186,19 +213,18 @@ lemma R3c_monotonic:
   by (utp_pred_tac)
 
 lemma R1_R3c_commute: "`R1(R3c(P))` =`R3c(R1(P))`"
-  apply(simp add:R3c_def SkipR_as_SkipRA)
-  apply(subst SkipRA_unfold_aux_ty[of "tr "], simp_all add:closure typing)
-  apply(subst SkipRA_unfold_aux_ty[of "tr "], simp_all add:closure typing) back
-  apply(utp_poly_auto_tac)
-done
+  proof-
+  have "`R1(R3c(P))` = `R1 (CSP1 (($tr\<acute> = $tr) \<and> II\<^bsub>REL_VAR - TR\<^esub>) \<lhd> $wait \<rhd> P)`"
+    by(simp add:R3c_def SkipR_as_SkipRA closure typing SkipRA_unfold_aux_ty[of "tr"])
+  also have "... = `CSP1 (($tr\<acute> = $tr) \<and> II\<^bsub>REL_VAR - TR\<^esub>) \<lhd> $wait \<rhd> R1 (P)`"  
+    by(utp_poly_auto_tac)
+  also have "... = `R3c(R1(P))`"
+    by(simp add:R3c_def SkipRA_unfold_aux_ty[of "tr "] SkipR_as_SkipRA closure typing) 
+  finally show ?thesis .
+qed
 
 lemma R2_R3c_commute: "`R2(R3c(P))` =`R3c(R2(P))`"
-  apply(simp add:R3c_def SkipR_as_SkipRA)
-  apply(subst SkipRA_unfold_aux_ty[of "tr "], simp_all add:closure typing)
-  apply(subst SkipRA_unfold_aux_ty[of "tr "], simp_all add:closure typing) back
-  apply(simp add:CSP1_def R2_def R2s_def usubst typing defined closure R1_OrP R1_CondR R1_extend_AndP[THEN sym])
-  apply(simp add:R1_def tr_prefix_as_nil)
-  done
+  by(simp add:R3c_def R2_CondR R2s_def usubst typing defined closure CSP1_R2_commute[THEN sym] SkipRA_is_R2)
 
 lemma R3c_AndP: 
   "`R3c(P \<and> Q)` = `R3c(P) \<and> R3c(Q)`"
@@ -213,10 +239,13 @@ lemma R3c_CondR:
   by utp_pred_auto_tac
 
 lemma R3c_form : "`R3c(P)` = `(\<not>$ok \<and> $wait \<and> ($tr \<le> $tr\<acute>)) \<or> ($ok \<and> $wait  \<and> II) \<or> (\<not>$wait \<and> P \<^sub>f)`"
-apply(simp add:R3c_def CondR_def)
-apply(subst NotP_PVarPE_PSubstPE,simp_all add:typing CSP1_R1_form_2 R1_SkipR is_healthy_def)
-apply (utp_poly_auto_tac)
-done
+proof -
+have "`R3c(P)` =  `($wait \<and> CSP1 ($ok \<and> II)) \<or> (\<not> $wait \<and> P)`"
+by(simp add:R3c_def CondR_def NotP_PVarPE_PSubstPE[THEN sym] typing CSP1_R1_form_2 R1_SkipR is_healthy_def)
+also have "... = `(\<not>$ok \<and> $wait \<and> ($tr \<le> $tr\<acute>)) \<or> ($ok \<and> $wait  \<and> II) \<or> (\<not>$wait \<and> P \<^sub>f)`"
+by (utp_poly_auto_tac)
+finally show ?thesis .
+qed
 
 lemma CSP1_R1_R3c_compose: 
   assumes "P is R1"
@@ -225,11 +254,7 @@ lemma CSP1_R1_R3c_compose:
 
 lemma CSP1_R3_ok': 
 "`CSP1($ok\<acute> \<and> R3c(P))` = `CSP1(R3c($ok\<acute> \<and> P))`"
-  apply (simp add:R3c_form CSP1_def SkipR_as_SkipRA)
-  apply (subst SkipRA_unfold_aux_ty[of "ok"],simp_all add:closure typing)
-  apply (subst SkipRA_unfold_aux_ty[of "ok"],simp_all add:closure typing) back
-  apply (utp_poly_auto_tac)
-done
+  by (simp add:R3c_form CSP1_def SkipR_as_SkipRA SkipRA_unfold_aux_ty[of "ok" "REL_VAR"] closure typing usubst,utp_poly_auto_tac)
 
 lemma R3c_seq_comp_1: 
   assumes "Q is R3c" "Q is R1" "Q \<in> WF_RELATION"
@@ -237,16 +262,13 @@ lemma R3c_seq_comp_1:
 proof -
   have "`(\<not>$ok \<and> $wait \<and> ($tr \<le> $tr\<acute>));Q` = `(\<not>$ok \<and> $wait \<and> ($tr \<le> $tr\<acute>));R1(R3c(Q))`"
     by(metis assms is_healthy_def)
+  also have "... = `\<not>$ok \<and> $wait \<and> ($tr \<le> $tr\<acute>);R1(R3c(Q))`"
+    by(simp add: SemiR_AndP_left_precond closure typing defined assms)
   also have "... = `\<not>$ok \<and> $wait \<and> (
                        ($tr \<le> $tr\<acute>) ; (\<not>$ok \<and> $wait \<and> ($tr \<le> $tr\<acute>)) \<or>
                        ($tr \<le> $tr\<acute>) ; ($ok \<and> $wait \<and> ($ok\<acute>=$ok) \<and> ($wait\<acute>=$wait) \<and> II\<^bsub>REL_VAR - {ok\<down>, ok\<down>\<acute>} - {wait\<down>, wait\<down>\<acute>}\<^esub> \<and> ($tr \<le> $tr\<acute>)) \<or>
                        ($tr \<le> $tr\<acute>) ; (\<not> $wait \<and> Q[false/wait] \<and> ($tr \<le> $tr\<acute>)))`"
-    apply(simp add: SemiR_AndP_left_precond closure typing defined assms)
-    apply(simp add:R1_def R3c_form SemiR_OrP_distl AndP_OrP_distr AndP_assoc[THEN sym] SkipR_as_SkipRA)
-    apply(subst SkipRA_unfold_aux_ty[of "ok"],simp_all add:typing closure)
-    apply(subst SkipRA_unfold_aux_ty[of "wait"],simp_all add:typing closure)
-    apply(simp add:AndP_assoc[THEN sym])
-    done
+    by(simp add:R1_def R3c_form SemiR_OrP_distl AndP_OrP_distr SkipR_as_SkipRA  SkipRA_unfold_aux_ty[of "ok" "REL_VAR"]  SkipRA_unfold_aux_ty[of "wait" "REL_VAR - OKAY"] typing closure AndP_assoc[THEN sym])
   also have "... = `\<not>$ok \<and> $wait \<and> (
                        ($tr \<le> $tr\<acute>) ; (\<not>$ok \<and> $wait \<and> ($tr \<le> $tr\<acute>)) \<or>
                        ($tr \<le> $tr\<acute>) ; (($ok \<and> $wait \<and> $ok\<acute> \<and> $wait\<acute>) \<and> II\<^bsub>REL_VAR - {ok\<down>, ok\<down>\<acute>} - {wait\<down>, wait\<down>\<acute>}\<^esub> \<and> ($tr \<le> $tr\<acute>)) \<or>
@@ -259,29 +281,16 @@ proof -
    qed
  also have "... = `\<not>$ok \<and> $wait \<and> (
                        ($tr \<le> $tr\<acute>) ; ($tr \<le> $tr\<acute>) \<or>
+                       ($tr \<le> $tr\<acute>) ; ($ok \<and> $wait \<and> $ok\<acute> \<and> $wait\<acute> \<and> II\<^bsub>REL_VAR - {ok\<down>, ok\<down>\<acute>} - {wait\<down>, wait\<down>\<acute>}\<^esub> \<and> ($tr \<le> $tr\<acute>)) \<or>
+                       ($tr \<le> $tr\<acute>) ; (Q[false/wait] \<and> ($tr \<le> $tr\<acute>)))`"
+    by(simp add:AndP_assoc[THEN sym] SemiR_remove_middle_unrest1[of "`$tr\<le>$tr\<acute>`" "`$wait \<and> ($tr\<le>$tr\<acute>)`" "{ok \<down>}" "`\<not>$ok`"] SemiR_remove_middle_unrest1[of "`$tr\<le>$tr\<acute>`" "`Q[false/wait] \<and> ($tr\<le>$tr\<acute>)`" "{wait \<down>}" "`\<not>$wait`"] SemiR_remove_middle_unrest1[of "`$tr\<le>$tr\<acute>`" "`($tr\<le>$tr\<acute>)`" "{wait \<down>}" "`$wait`"] typing closure defined unrest assms)
+ also have "... = `\<not>$ok \<and> $wait \<and> (
+                       ($tr \<le> $tr\<acute>) ; ($tr \<le> $tr\<acute>) \<or>
                        ($tr \<le> $tr\<acute>) ; ($ok\<acute> \<and> $wait\<acute> \<and> II\<^bsub>REL_VAR - {ok\<down>, ok\<down>\<acute>} - {wait\<down>, wait\<down>\<acute>}\<^esub> \<and> ($tr \<le> $tr\<acute>)) \<or>
                        ($tr \<le> $tr\<acute>) ; (Q[false/wait] \<and> ($tr \<le> $tr\<acute>)))`"
-    apply(simp add:AndP_assoc[THEN sym])
-    apply(simp add: SemiR_remove_middle_unrest1[of _ _ "{ok \<down>}"] typing closure defined unrest assms)
-    apply(simp add: SemiR_remove_middle_unrest1[of _ _ "{wait \<down>}"] typing closure defined unrest assms)
-    apply(subst SemiR_remove_middle_unrest1[of _ _ "{ok \<down>}"],simp_all add: typing closure defined unrest)
-defer 
-apply(utp_poly_auto_tac)
-apply(rule unrest) back back
-apply(simp_all add:unrest closure typing)
-apply(rule unrest) back back
-apply(simp_all add:unrest closure typing)
-apply(rule unrest) back back
-apply(simp_all add:unrest closure typing)
-apply(rule unrest) back back
-apply(subst UNREST_subset)
-apply(subst UNREST_SkipRA)
-apply(simp_all add:typing closure defined unrest) 
-done
+    by(utp_poly_auto_tac)
 also have "... = `\<not>$ok \<and> $wait \<and> ($tr \<le> $tr\<acute>);((true \<or> ($ok\<acute> \<and> $wait\<acute> \<and> II\<^bsub>REL_VAR - {ok \<down>,ok \<down>\<acute>} - {wait \<down>,wait \<down>\<acute>}\<^esub>) \<or> Q[false/wait]) \<and> ($tr \<le> $tr\<acute>))`"
-apply(subst AndP_OrP_distr)
-apply(simp add:AndP_OrP_distr SemiR_OrP_distl AndP_assoc[THEN sym])
-done
+  by(utp_poly_auto_tac)
 also have "... = `\<not>$ok \<and> $wait \<and> ($tr \<le> $tr\<acute>)`"
   by(simp add:utp_pred_simps(8) tr_leq_trans)
   finally show ?thesis
@@ -293,11 +302,7 @@ lemma R3c_seq_comp_2:
   shows "`($ok \<and> $wait \<and> II);Q` = `$ok \<and> $wait \<and> II`"
 proof -
   have "`($ok \<and> $wait \<and> II);Q` =`($ok \<and> $wait \<and> II\<^bsub>REL_VAR - OKAY - {wait \<down>,wait \<down>\<acute>}\<^esub>);($ok \<and> $wait \<and> Q)`"
-    apply(simp add:SkipR_as_SkipRA SemiR_AndP_right_precond typing closure urename assms AndP_assoc[THEN sym])
-    apply(subst SkipRA_unfold_aux_ty[of "ok"], simp_all add:closure typing)
-    apply(subst SkipRA_unfold_aux_ty[of "wait"], simp_all add:closure typing)
-    apply(utp_poly_auto_tac)
-    done
+    by(simp add:SkipR_as_SkipRA SemiR_AndP_right_precond urename assms AndP_assoc[THEN sym] SkipRA_unfold_aux_ty[of "ok" "REL_VAR"] SkipRA_unfold_aux_ty[of "wait" "REL_VAR - OKAY"] closure typing, utp_poly_auto_tac)
   also have "... = `($ok \<and> $wait \<and> II\<^bsub>REL_VAR - OKAY - {wait \<down>,wait \<down>\<acute>}\<^esub>);($ok \<and> $wait \<and> R3c(Q))`"
     proof -
       have 1: "Q = `R3c(Q)`"
@@ -306,17 +311,11 @@ proof -
         by(subst 1,simp)
     qed
   also have "... = `($ok \<and> $wait \<and> II\<^bsub>REL_VAR - OKAY - {wait \<down>,wait \<down>\<acute>}\<^esub>);($ok \<and> $wait \<and> II)`"
-    apply(simp add:R3c_def CSP1_def)
-    apply(utp_poly_auto_tac)
-    done
+    by(utp_poly_auto_tac)
   also have "... = `($ok \<and> $wait \<and> II\<^bsub>REL_VAR - OKAY - {wait \<down>,wait \<down>\<acute>}\<^esub> \<and> $ok\<acute> \<and> $wait\<acute>)`"
     by(simp add:SemiR_AndP_right_precond assms closure typing urename AndP_assoc[THEN sym])
   also have "... = `$ok \<and> $wait \<and> II`"
-    apply(simp add:SkipR_as_SkipRA)
-    apply(subst SkipRA_unfold_aux_ty[of "ok"], simp_all add:closure typing) back
-    apply(subst SkipRA_unfold_aux_ty[of "wait"], simp_all add:closure typing) back
-    apply(utp_poly_auto_tac)
-    done
+    by(simp add:SkipR_as_SkipRA SkipRA_unfold_aux_ty[of "ok" "REL_VAR"] SkipRA_unfold_aux_ty[of "wait" "REL_VAR - OKAY"] closure typing,utp_poly_auto_tac)
   finally show ?thesis
     by this
 qed
@@ -326,12 +325,10 @@ lemma R3c_SemiR_closure:
   shows " `P ; Q` is R3c"
 proof -
 have "`P;Q` = `R3c(P);Q`"by(metis assms is_healthy_def)
+also have "... = `(\<not> $ok \<and> $wait \<and> ($tr \<le> $tr\<acute>)) \<or> ($ok \<and> $wait \<and> II) \<or> (\<not> $wait \<and> P[false/wait]) ; Q `"
+   by(simp add:R3c_form SemiR_OrP_distr R3c_seq_comp_1 assms R3c_seq_comp_2)
 also have "... = `R3c(P;Q)`"
-   apply(simp add:R3c_form)
-   apply(subst SubstP_SemiR_left,simp_all add:typing defined closure unrest)
-   apply(simp add: SemiR_OrP_distr R3c_seq_comp_1 assms R3c_seq_comp_2)
-   apply(subst SemiR_AndP_left_precond,simp_all add:typing closure defined unrest assms)
-   done
+   by(simp add: SemiR_AndP_left_precond typing closure defined unrest assms R3c_form SubstP_SemiR_left)
 finally show ?thesis by (metis is_healthy_def)
 qed
 
